simulation/correct_get_addr_ofs.v
@@ -1,50 +1,55 @@
 From bpf.comm Require Import State Monad.
-From bpf.src Require Import DxValues DxInstructions.
-From Coq Require Import List Lia ZArith.
+From bpf.monadicmodel Require Import rBPFInterpreter.
+From Coq Require Import List Lia.
 From compcert Require Import Integers Values Clight Memory.
 Import ListNotations.
+Require Import ZArith.
 
 From bpf.proof Require Import Clightlogic MatchState CorrectRel CommonLemma.
 
 From bpf.clight Require Import interpreter.
 
 
-
 (**
+unsigned int get_addr_ofs(unsigned long long x, int ofs)
+{
+  return (unsigned int) (x + (unsigned long long) ofs);
+}
 
-Print get_sub.
-get_sub = 
-fun x y : valu32_t => returnM (Val.sub x y)
-     : valu32_t -> valu32_t -> M valu32_t
+Print get_addr_ofs.
+get_addr_ofs = 
+fun (x : val64_t) (ofs : sint32_t) =>
+returnM (val_intuoflongu (Val.addl x (Val.longofintu (sint32_to_vint ofs))))
+     : val64_t -> sint32_t -> M valu32_t
 
 *)
 
-Section Get_sub.
+Section Get_addr_ofs.
 
   (** The program contains our function of interest [fn] *)
   Definition p : Clight.program := prog.
 
   (* [Args,Res] provides the mapping between the Coq and the C types *)
   (* Definition Args : list CompilableType := [stateCompilableType].*)
-  Definition args : list Type := [(valu32_t:Type); (valu32_t:Type)].
-  Definition res : Type := (valu32_t:Type).
+  Definition args : list Type := [(val:Type); (int:Type)].
+  Definition res : Type := (val:Type).
 
   (* [f] is a Coq Monadic function with the right type *)
-  Definition f : arrow_type args (M res) := get_sub.
+  Definition f : arrow_type args (M res) := get_addr_ofs.
 
   (* [fn] is the Cligth function which has the same behaviour as [f] *)
-  Definition fn: Clight.function := f_get_sub.
+  Definition fn: Clight.function := f_get_addr_ofs.
 
   (* [match_arg] relates the Coq arguments and the C arguments *)
   Definition match_arg_list : DList.t (fun x => x -> val -> State.state -> Memory.Mem.mem -> Prop) args :=
-    (DList.DCons (stateless valu32_correct)
-       (DList.DCons (stateless valu32_correct)
+    (DList.DCons (stateless val64_correct)
+       (DList.DCons (stateless sint32_correct)
                     (DList.DNil _))).
 
   (* [match_res] relates the Coq result and the C result *)
   Definition match_res : res -> val -> State.state -> Memory.Mem.mem -> Prop := fun x v st m => valu32_correct x v.
 
-  Instance correct_function3_get_sub : forall a, correct_function3 p args res f fn (nil) true match_arg_list match_res a.
+  Instance correct_function3_get_addr_ofs : forall a, correct_function3 p args res f fn (nil) true match_arg_list match_res a.
   Proof.
     correct_function_from_body args.
     correct_body.
@@ -53,19 +58,22 @@ Section Get_sub.
     unfold f.
     repeat intro.
     get_invariant_more _x.
-    get_invariant_more _y.
+    get_invariant_more _ofs.
 
-    unfold stateless, valu32_correct in H0, H2.
-    destruct H0 as (Hc_eq & vi & Hvi_eq).
-    destruct H2 as (Hc0_eq & vj & Hvj_eq).
-    subst.
+    unfold stateless, val64_correct in H0.
+    unfold stateless, sint32_correct in H2.
+    destruct H0 as (Hc_eq & (vi & Hvi_eq)).
+    subst c v v0.
 
     (**according to the type of eval_pc:
-         static unsigned long long get_subl(unsigned long long x1, unsigned long long y1)
+unsigned int get_addr_ofs(unsigned long long x, int ofs)
+{
+  return (unsigned int) (x + (unsigned long long) ofs);
+}
        1. return value should be  x+y
        2. the memory is same
       *)
-    exists (Val.sub (Vint vi) (Vint vj)), m, Events.E0.
+    eexists. exists m, Events.E0.
 
     repeat split; unfold step2.
     -
@@ -77,6 +85,6 @@ Section Get_sub.
       reflexivity.
   Qed.
 
-End Get_sub.
+End Get_addr_ofs.
 
-Existing Instance correct_function3_get_sub.
+Existing Instance correct_function3_get_addr_ofs.
