simulation/correct_get_block_ptr.v
@@ -1,5 +1,5 @@
 From bpf.comm Require Import MemRegion State Monad.
-From bpf.src Require Import DxValues DxInstructions.
+From bpf.monadicmodel Require Import rBPFInterpreter.
 From dx.Type Require Import Bool.
 From dx Require Import IR.
 From Coq Require Import List ZArith.
@@ -13,13 +13,12 @@ From bpf.clight Require Import interpreter.
 
 
 (**
-Check get_block_perm.
-
-get_block_perm
-     : memory_region -> DxMonad.M permission
+Check get_block_ptr.
+get_block_ptr
+     : memory_region -> M val64_t
 *)
 
-Section Get_block_perm.
+Section Get_block_ptr.
 
   (** The program contains our function of interest [fn] *)
   Definition p : Clight.program := prog.
@@ -27,17 +26,17 @@ Section Get_block_perm.
   (* [Args,Res] provides the mapping between the Coq and the C types *)
   (* Definition Args : list CompilableType := [stateCompilableType].*)
   Definition args : list Type := [(memory_region:Type)].
-  Definition res : Type := (permission:Type).
+  Definition res : Type := (val:Type).
 
   (* [f] is a Coq Monadic function with the right type *)
-  Definition f : arrow_type args (M res) := get_block_perm.
+  Definition f : arrow_type args (M res) := get_block_ptr.
 
   Variable state_block: block. (**r a block storing all rbpf state information? *)
   Variable mrs_block: block.
   Variable ins_block: block.
 
   (* [fn] is the Cligth function which has the same behaviour as [f] *)
-  Definition fn: Clight.function := f_get_block_perm.
+  Definition fn: Clight.function := f_get_block_ptr.
 
   (* [match_arg] relates the Coq arguments and the C arguments *)
   Definition match_arg_list : DList.t (fun x => x -> val -> State.state -> Memory.Mem.mem -> Prop) args :=
@@ -45,9 +44,9 @@ Section Get_block_perm.
        (DList.DNil _)).
 
   (* [match_res] relates the Coq result and the C result *)
-  Definition match_res : res -> val -> State.state -> Memory.Mem.mem -> Prop := fun x v st m => perm_correct x v.
+  Definition match_res : res -> val -> State.state -> Memory.Mem.mem -> Prop := fun x v st m => val_ptr_correct x v.
 
-  Instance correct_function3_get_block_perm : forall a, correct_function3 p args res f fn (nil) true match_arg_list match_res a.
+  Instance correct_function3_get_block_ptr : forall a, correct_function3 p args res f fn (nil) true match_arg_list match_res a.
   Proof.
     correct_function_from_body args.
     correct_body.
@@ -57,35 +56,31 @@ Section Get_block_perm.
     repeat intro.
     get_invariant_more _mr.
 
-    unfold my_match_region in H0.
+    unfold match_region, my_match_region in H0.
     destruct H0 as (o & Hptr & Hmatch).
     unfold match_region_at_ofs in Hmatch.
-    destruct Hmatch as (_ & _ & (vperm & Hperm_load & Hinj) & _).
+    destruct Hmatch as (_ & _ & _ & (b & ofs & Hptr_load & Hinj)).
     subst.
 
-    (**according to the type:
-         static unsigned long long getMemRegion_start_addr(struct memory_region *mr1)
-       1. return value should be  `Vlong vaddr`
-       2. the memory is same
-      *)
-    exists (Vint vperm), m, Events.E0.
+    exists (Vptr b ofs), m, Events.E0.
 
     repeat split; unfold step2.
     -
       repeat forward_star.
-      unfold align, Ctypes.alignof; simpl.
-      unfold Mem.loadv in Hperm_load.
-      rewrite Hperm_load; reflexivity.
-
+      simpl.
       Transparent Archi.ptr64.
+      unfold align, Ctypes.align_attr; simpl.
+      unfold Mem.loadv in Hptr_load.
+      rewrite Hptr_load; reflexivity.
+
+      simpl.
       reflexivity.
-    - unfold match_res. unfold correct_perm in Hinj. unfold perm_correct. 
-      destruct (block_perm c); rewrite Hinj; reflexivity.
+    - assumption.
+    - exists b, ofs; assumption.
     - simpl.
       constructor.
-      reflexivity.
   Qed.
 
-End Get_block_perm.
+End Get_block_ptr.
 
-Existing Instance correct_function3_get_block_perm.
+Existing Instance correct_function3_get_block_ptr.
