simulation/correct_get_opcode_branch.v
@@ -1,6 +1,5 @@
 From bpf.comm Require Import Regs State Monad.
-From bpf.src Require Import DxNat DxOpcode DxIntegers DxInstructions.
-From bpf.monadicmodel Require Import Opcode.
+From bpf.monadicmodel Require Import Opcode rBPFInterpreter.
 From Coq Require Import List Lia ZArith.
 From compcert Require Import Integers Values Clight Memory.
 Import ListNotations.
@@ -24,7 +23,7 @@ Section Get_opcode_branch.
 
   (* [Args,Res] provides the mapping between the Coq and the C types *)
   (* Definition Args : list CompilableType := [stateCompilableType].*)
-  Definition args : list Type := [(nat8:Type)].
+  Definition args : list Type := [(nat:Type)].
   Definition res : Type := (opcode_branch:Type).
 
   (* [f] is a Coq Monadic function with the right type *)
@@ -39,7 +38,7 @@ Section Get_opcode_branch.
 
   (* [match_arg] relates the Coq arguments and the C arguments *)
   Definition match_arg_list : DList.t (fun x => x -> val -> State.state -> Memory.Mem.mem -> Prop) args :=
-    (DList.DCons (stateless opcode_alu64_nat8_correct)
+    (DList.DCons (stateless opcode_and_07_correct)
                 (DList.DNil _)).
 
   (* [match_res] relates the Coq result and the C result *)
@@ -55,8 +54,8 @@ Section Get_opcode_branch.
     repeat intro.
     get_invariant_more _op.
 
-    unfold stateless, opcode_alu64_nat8_correct in H0.
-    destruct H0 as (H0 & Hland & Hge).
+    unfold stateless, opcode_and_07_correct in H0.
+    destruct H0 as (H0 & Hge).
     subst.
 
     eexists. exists m, Events.E0.
@@ -70,7 +69,10 @@ Section Get_opcode_branch.
       unfold match_res, opcode_branch_correct.
       rewrite byte_to_opcode_branch_if_same.
       unfold byte_to_opcode_branch_if.
-      rewrite Int.zero_ext_and; [simpl | lia].
+      assert (H255_eq: (two_p 8 - 1 = 255)%Z). {
+        reflexivity.
+      }
+      rewrite Int.zero_ext_and; [rewrite H255_eq | lia].
       rewrite nat8_land_240_255_eq; [| apply Hge].
 
 Ltac simpl_if Ht :=
@@ -79,10 +81,27 @@ Ltac simpl_if Ht :=
     destruct X eqn: Ht; [rewrite Nat.eqb_eq in Ht | rewrite Nat.eqb_neq in Ht]
   end.
 
-Ltac simpl_alu_opcode Hop := simpl_if Hop; [rewrite Hop; reflexivity | ].
+Ltac simpl_alu_opcode Hop := simpl_if Hop; [rewrite Hop; intuition | ].
 
       simpl_if Hja.
-      destruct (c =? 5)%nat eqn: Hc_eq; [rewrite Nat.eqb_eq in Hc_eq; rewrite Hc_eq; reflexivity | eexists; reflexivity].
+      destruct (c =? 5)%nat eqn: Hc_eq; [rewrite Nat.eqb_eq in Hc_eq; rewrite Hc_eq; exists; reflexivity |rewrite Nat.eqb_neq in Hc_eq].
+      exists c; split; [reflexivity| idtac].
+      unfold is_illegal_jmp_ins.
+      split.
+      intro.
+      assumption.
+Ltac simpl_land HOP:=
+  match goal with
+  | H: Nat.land ?X ?Y = ?Z |- (Nat.land ?X ?Y <> ?W) /\ _ =>
+      split; [intro HOP; rewrite H in HOP; inversion HOP |]
+  | H: Nat.land ?X ?Y = ?Z |- (Nat.land ?X ?Y = ?W -> _) /\ _ =>
+      split; [intro HOP; rewrite H in HOP; inversion HOP |]
+  | H: Nat.land ?X ?Y = ?Z |- (Nat.land ?X ?Y <> ?W) =>
+      intro HOP; rewrite H in HOP; inversion HOP
+  | H: Nat.land ?X ?Y = ?Z |- (Nat.land ?X ?Y = ?W -> _) =>
+      intro HOP; rewrite H in HOP; inversion HOP
+  end.
+      repeat simpl_land H0.
       simpl_alu_opcode Hjeq.
       simpl_alu_opcode Hjgt.
       simpl_alu_opcode Hjge.
@@ -95,8 +114,21 @@ Ltac simpl_alu_opcode Hop := simpl_if Hop; [rewrite Hop; reflexivity | ].
       simpl_alu_opcode Hjsjt.
       simpl_alu_opcode Hjsle.
       simpl_if Hret.
-      destruct (c =? 149)%nat eqn: Hc_eq; [rewrite Nat.eqb_eq in Hc_eq; rewrite Hc_eq; reflexivity | eexists; reflexivity].
-      eexists; reflexivity.
+      destruct (c =? 149)%nat eqn: Hc_eq; [rewrite Nat.eqb_eq in Hc_eq; rewrite Hc_eq; exists; reflexivity | rewrite Nat.eqb_neq in Hc_eq].
+      exists c; split; [reflexivity| ].
+      unfold is_illegal_jmp_ins.
+      repeat simpl_land H0.
+      assumption.
+      exists c.
+      split; [reflexivity |].
+      unfold is_illegal_jmp_ins.
+      repeat split; try assumption.
+      intro.
+      rewrite H0 in Hja.
+      exfalso; apply Hja; reflexivity.
+      intro.
+      rewrite H0 in Hret.
+      exfalso; apply Hret; reflexivity.
     - simpl.
       constructor.
       rewrite Int.zero_ext_idem;[idtac | lia].
