simulation/correct_upd_pc.v
@@ -1,5 +1,5 @@
 From bpf.comm Require Import State Monad.
-From bpf.src Require Import DxIntegers DxInstructions.
+From bpf.monadicmodel Require Import rBPFInterpreter.
 From Coq Require Import List Lia ZArith.
 From compcert Require Import Integers Values Clight Memory.
 Import ListNotations.
@@ -10,65 +10,67 @@ From bpf.clight Require Import interpreter.
 
 
 (**
-Check upd_pc_incr.
-upd_pc_incr
-     : M unit
+Check upd_pc.
+upd_pc
+     : sint32_t -> M unit
  *)
 
-Section Upd_pc_incr.
+Section Upd_pc.
 
   (** The program contains our function of interest [fn] *)
   Definition p : Clight.program := prog.
 
   (* [Args,Res] provides the mapping between the Coq and the C types *)
   (* Definition Args : list CompilableType := [stateCompilableType].*)
-  Definition args : list Type := [].
+  Definition args : list Type := [(int:Type)].
   Definition res : Type := unit.
 
   (* [f] is a Coq Monadic function with the right type *)
-  Definition f : arrow_type args (M res) := Monad.upd_pc_incr.
+  Definition f : arrow_type args (M res) := Monad.upd_pc.
 
   Variable state_block: block. (**r a block storing all rbpf state information? *)
   Variable mrs_block: block.
   Variable ins_block: block.
 
   (* [fn] is the Cligth function which has the same behaviour as [f] *)
-  Definition fn: Clight.function := f_upd_pc_incr.
+  Definition fn: Clight.function := f_upd_pc.
 
   Definition modifies : list block := [state_block]. (* of the C code *)
-  (* [match_mem] related the Coq monadic state and the C memory *)
-  (*Definition match_mem : stateM -> val -> Memory.Mem.mem -> Prop := fun stM v m => match_meminj_state state_block inject_id stM m.*)
-
-
+  
   Definition stateM_correct (st:unit) (v: val) (stm:State.state) (m: Memory.Mem.mem) :=
     v = Vptr state_block Ptrofs.zero /\ match_state state_block mrs_block ins_block stm m.
 
   (* [match_arg] relates the Coq arguments and the C arguments *)
   Definition match_arg_list : DList.t (fun x => x -> val -> State.state -> Memory.Mem.mem -> Prop) ((unit:Type) ::args) :=
-    DList.DCons stateM_correct (DList.DNil _).
+    DList.DCons stateM_correct
+                (DList.DCons (stateless sint32_correct)
+                             (DList.DNil _)).
 
   (* [match_res] relates the Coq result and the C result *)
   Definition match_res : res -> val -> State.state -> Memory.Mem.mem -> Prop := fun _ v st m => match_state state_block mrs_block ins_block st m /\ v = Vundef.
 
-  Lemma correct_function3_upd_pc_incr : forall a, correct_function3 p args res f fn modifies false match_arg_list match_res a.
+  Instance correct_function3_upd_pc : forall a, correct_function3 p args res f fn modifies false match_arg_list match_res a.
   Proof.
     correct_function_from_body args.
     correct_body.
     repeat intro.
     unfold INV in H.
-    get_invariant _st.
-    destruct c as (H_st & Hst_casted).
-    unfold stateM_correct in H_st.
-    destruct H_st as (Hv_eq & Hst).
+    get_invariant_more _st.
+    get_invariant_more _pc.
+    unfold stateM_correct in H0.
+    unfold stateless, sint32_correct in H2.
+    destruct H0 as (Hv_eq & Hst).
+    (*pose (mpc_store state_block st m Hst c (bpf_m st)). *)   
     subst.
-
-    (** we need to get the proof of `upd_pc_incr` load/store permission *)
-    apply (upd_pc_store _ _ _ _ (Int.add (pc_loc st) (Int.repr 1)) _) in Hst as Hstore.
+    
+    (** we need to get the proof of `upd_pc` store permission *)
+    apply (upd_pc_store _ _ _ _ c _) in Hst as Hstore.
     destruct Hstore as (m1 & Hstore).
     (** pc \in [ (state_block,0), (state_block,8) ) *)
 
-    (**according to the type of upd_pc_incr:
-         static void upd_pc_incr(struct bpf_state* st) 
+    simpl in c.
+    (**according to the type of upd_pc:
+         static void upd_pc(struct bpf_state* st, unsigned long long pc)
        1. return value should be Vundef (i.e. void)
        2. the new memory should change the value of pc, i.e. m_pc
       *)
@@ -77,24 +79,16 @@ Section Upd_pc_incr.
     split; unfold step2.
     - (* goal: Smallstep.star  _ _ (State _ (Ssequence ... *)
       repeat forward_star.
-
-      rewrite Ptrofs.add_zero.
-      destruct Hst as (_ , Hpc, _, _, _, _, _, _, _, _).
-      fold Ptrofs.zero in Hpc.
-      rewrite Hpc; reflexivity.
-      reflexivity.
-      reflexivity.
     - split.
       split.
       eapply upd_pc_preserves_match_state.
       apply Hst.
-      unfold State.upd_pc, State.upd_pc_incr.
       reflexivity.
       apply Hstore.
       reflexivity.
 
+      split.
       simpl.
-      constructor.
       constructor.
 
       unfold unmodifies_effect, modifies, In.
@@ -110,6 +104,6 @@ Section Upd_pc_incr.
       left; assumption.
 Qed.
 
-End Upd_pc_incr.
+End Upd_pc.
 
-Existing Instance correct_function3_upd_pc_incr.
+Existing Instance correct_function3_upd_pc.
