proof/CommonLemmaNat.v
@@ -1,5 +1,4 @@
 From compcert Require Import Integers.
-From bpf.src Require Import DxOpcode.
 From bpf.monadicmodel Require Import Opcode.
 From Coq Require Import Lia ZArith.
 
