simulation/correct_is_well_chunk_bool.v
@@ -1,5 +1,5 @@
 From bpf.comm Require Import rBPFAST State Monad.
-From bpf.src Require Import DxValues DxInstructions.
+From bpf.monadicmodel Require Import rBPFInterpreter.
 From dx.Type Require Import Bool.
 From dx Require Import IR.
 From Coq Require Import List ZArith.
