simulation/correct_upd_flag.v
@@ -1,5 +1,5 @@
 From bpf.comm Require Import Flag State Monad.
-From bpf.src Require Import DxValues DxInstructions.
+From bpf.monadicmodel Require Import rBPFInterpreter.
 From Coq Require Import List Lia ZArith.
 From compcert Require Import Integers Values Clight Memory.
 Import ListNotations.
